theories/cancellation/CancelPrepare.v
@@ -1,0 +1,191 @@
+From CRIS.simulations.gsim Require Import GSimAux.
+From CRIS.simulations.msim Require Import MSimCommon ISim ISimRefl WSim WSimFacts Tactics TacticsInit.
+
+Section PREPARE_SIM.
+
+  Context `{!crisG Γ Σ α β τ _S _I}.
+
+  Theorem prepare_sim (spt sps: specmap) (md: SMod.t)
+    (SP1: ∀ fn arg (msk: emask) p, md.(SMod.fnsems) !! fn = Some (Some (msk,p)) →
+          ∀ (fc: string), spt.1 !! (funid fc) ≠ sps.1 !! (funid fc) →
+          msk _ (subevent _ (Call fc arg)) = false ∧
+          msk _ (subevent _ (Spawn fc arg)) = false)
+    (SPS: sps.2 = true)
+    (SP2: spt.2 = false →
+          ∀ fn (msk: emask) p, md.(SMod.fnsems) !! fn = Some (Some (msk,p)) →
+          ∀ T (e: callE T), msk_sys _ (subevent _ e) = true → msk _ (subevent _ e) = false)
+    :
+    ⊢ ISim.t open (SMod.to_mod_cancel sps md) (SMod.to_mod spt md) (IstEq (SMod.to_mod spt md)).
+  Proof.
+    cStartModSim; et.
+    iApply (state_eq_init_same with "SRC TGT").
+
+    { destruct Hwf as [Hwf _]. rewrite /Mod.fnsems in Hwf |- *; ss.
+      ii. specialize (Hwf i x). revert Hwf H. rewrite !lookup_fmap. i.
+      destruct (SMod.fnsems md !! i) eqn: Emd; ss. depdes H. destruct o; ss. et. }
+
+    rewrite /ISim.sim_fun.
+    iIntros (STATE).
+    iIntros "%WFS %WFT" (fs) "%Hfs".
+    simpl_map. des_ifs; ss.
+    rewrite /SMod.to_mod_cancel /SMod.to_mod /Mod.fnsems
+      /sandbox_fnsemmap /IstEq !lookup_fmap in Hfs |- *. s.
+    do 2 (rewrite fmap_Some in Hfs; des); subst.
+    destruct x0 as [[msk [fspo fbd]]|]; ss.
+    depdes Hfs0. rewrite Hfs. s. clarify.
+    hexploit (SMod.well_scoped_fns md fn (msk, (fspo, fbd))).
+    { rewrite lookup_omap Hfs //. }
+    intros [HPUT HGET].
+    iExists _. iSplit; first done.
+    rewrite /isim_fsem.
+    iIntros "!#" (arg) "IST"; iApply wsim_isim;
+    rewrite /SB.sandbox_body;
+    simpl fst; simpl snd; rewrite /SModTr.trans_fnsem /SModTr.HoareFun /cfunU /cfunN.
+    iStopProof.
+    match goal with
+      |- ?P ⊢ wsim ?fe_s ?fe_t ?Ist ?E ?g _ _ ?rel _ _ _ _ =>
+      assert (HYP: ∀ ps pt itr, P ⊢ wsim fe_s fe_t Ist E g _ _ rel ps pt
+              (⇓sb(msk) (SModTr._trans sps (Some msk) itr))
+              (⇓sb(msk) (SModTr._trans spt None itr)))
+    end; cycle 1.
+    {
+      iIntros "IST". destruct fspo; cycle 1.
+      { cStepsS. cStepsT. iStopProof. eapply HYP. }
+      cStepsS. cStepsT. des_if; [| cStepsS; ss].
+      cStepsS. case_match; [| cStepsS; ss].
+      cStepsS. case_match; [| cStepsS; ss].
+      cStepsS. cForceT _q. cStepsT. rewrite H. cStepsT.
+      cForcesT. cStepsT. erewrite H0. cForcesT. iFrame.
+      cStepsT. cBind _ "IST" as (??) "Q".
+      { iStopProof. eapply HYP. }
+      iDestruct "Q" as "[-> IST]".
+      cStepsT. cStepsS. des_if; [| cStepsS; ss].
+      cStepsT. bsimpl. cStepsT. cForceS. cStepsS. bsimpl. cForceS. iFrame.
+      cStep. iSplit; first done. iFrame.
+    }
+
+    iIntros (???) "IST".
+    cCoind CIH g __ with ps pt itr. iIntros "IST".
+    assert (CASE := case_itrH itr); des; subst.
+    - rewrite !SRed._ret. cStep. iSplit; first done. iFrame.
+    - rewrite !SRed._tau. cStepsS. cStepsT.
+      cByCoind CIH; try et. iFrame "IST WINV".
+    - rewrite !SRed._bind !SRed._ag. cStepsS. cStepsT. des_if; [|cStepsS; ss].
+      cStepsS. cForceT. iFrame. cStepsT.
+      cByCoind CIH; try et. iFrame "IST WINV".
+    - rewrite !SRed._bind !SRed._ag. cStepsS. cStepsT. des_if; [|cStepsS; ss].
+      cStepsS. cForceT. iFrame. cStepsT.
+      cByCoind CIH; try et. iFrame "IST WINV".
+    - rewrite !SRed._bind !SRed._ag. cStepsS. cStepsT. des_if; [|cStepsS; ss].
+      cStepsT. cForceS. iFrame. cStepsS.
+      cByCoind CIH; try et. iFrame "IST WINV".
+    - destruct c.
+      + rewrite !SRed._bind !SRed._call. unfold SModTr.HoareCall. cStepsS. cStepsT.
+        case_match eqn: Lsps; cycle 1.
+        { case_match eqn: Lspt.
+          { hexploit (SP1 fn args); et.
+            { erewrite Lsps, Lspt. et. }
+            intros [Lmsk _]. cStepsS. rewrite Lmsk. cStepsS. ss.
+          }
+          cStepsS. cStepsT. des_if; [|cStepsS; ss].
+          cCall "IST" as (?) "IST". cStepsS. cStepsT.
+          cByCoind CIH; try et. iFrame "IST WINV".
+        }
+        destruct (spt.1 !! funid fn0) eqn: Lspt; cycle 1.
+        { hexploit (SP1 fn args); et.
+          { erewrite Lsps, Lspt. et. }
+          intros [Lmsk _]. rewrite Lmsk. cStepsS. bsimpl. cForceS (). cStepsS. bsimpl.
+          cForcesS. cStepsS. bsimpl. cForcesS. iSplit; et. cStepsS. rewrite Lmsk. cStepsS. ss.
+        }
+        destruct (classic (f = f0)) eqn: Ef_f0; cycle 1.
+        { hexploit (SP1 fn args); et.
+          { erewrite Lsps, Lspt. ii. depdes H. et. }
+          intros [Lmsk _]. rewrite Lmsk.
+          cStepsS. bsimpl. cForceS (). cStepsS. bsimpl. cForcesS. cStepsS.
+          bsimpl. cForcesS. iSplit; et. cStepsS. rewrite Lmsk. cStepsS. ss.
+        }
+        subst. case_match eqn: Lmsk; cycle 1.
+        { cStepsS. bsimpl. cForceS (). cStepsS. bsimpl. cForcesS. cStepsS.
+          bsimpl. cForcesS. iSplit; et. cStepsS. rewrite Lmsk. cStepsS. ss.
+        }
+        cNormS. cStepsT. bsimpl. cStepsT. cForceS _q. cStepsS. bsimpl.
+        cStepsT. cForceS _q0. cStepsS. bsimpl.
+        cStepsT. cForceS. iFrame. cStepsS. bsimpl. des_if; [|cStepsS; ss].
+        cCall "IST" as (?) "IST". cStepsS. cStepsT. des_if; [|cStepsS; ss].
+        cStepsS. cForceT _q1. cStepsT. des_if; [|cStepsS; ss].
+        cStepsS. cForceT. iFrame. cStepsT.
+        cByCoind CIH; try et. iFrame "IST WINV".
+      + rewrite !SRed._bind !SRed._spawn. cStepsS. cStepsT.
+        rewrite /SModTr.HoareSpawn !SPS.
+        destruct (classic (spt.1 !! funid fn0 = sps.1 !! funid fn0)) eqn: EQf_f0; cycle 1.
+        { hexploit (SP1 fn args); et.
+          intros [_ Lmsk]. destruct spt.2.
+          - cStepsS. bsimpl. cForceS args. cStepsS. rewrite Lmsk. cStepsS. ss.
+          - cStepsS. bsimpl. cForceS args. cStepsS. erewrite SP2; et. cStepsS. ss.
+        }
+        destruct spt.2; cycle 1.
+        { cStepsS. bsimpl. cForceS args. cStepsS. erewrite SP2; et. cStepsS. ss. }
+        cStepsS. cStepsT. bsimpl. cStepsT. cForceS _q. cStepsS. des_if; [|cStepsS; ss].
+        cStep. cStepsS. cStepsT. des_if; [|cStepsS; ss].
+        cStepsS. cForceT. iFrame. cStepsT. bsimpl.
+        cStepsT. rewrite -e. cForceS _q0. bsimpl.
+        cStepsT. cForceS. iFrame. cStepsS.
+        cByCoind CIH; try et. iFrame "IST WINV".
+      + rewrite !SRed._bind !SRed._yield. cStepsS. cStepsT. rewrite /SModTr.HoareYield.
+        rewrite SPS. s. destruct (msk _ _) eqn: Emsk; cycle 1.
+        { cStepsS. bsimpl. cForceS tid. cStepsS. bsimpl.
+          cForceS. iSplit; et. cStepsS. erewrite Emsk; et. cStepsS. ss.
+        }
+        destruct spt.2 eqn: Espt; cycle 1.
+        { erewrite SP2 in Emsk; et; ss. }
+        cStepsS. cStepsT. des_if; [|cStepsS; ss].
+        cStepsT. cForceS _q. cStepsS. bsimpl.
+        cStepsT. cForcesS. iFrame. cStepsS. des_if; [|cStepsS; ss].
+        cYield "IST" "IST". cStepsS. cStepsT. des_if; [|cStepsS; ss].
+        cStepsS. cForceT. iFrame. cStepsT.
+        cByCoind CIH; try et. iFrame "IST WINV".
+      + rewrite !SRed._bind !SRed._gettid. cStepsS. cStepsT. rewrite /SModTr.HoareGetTid.
+        rewrite SPS. s. destruct (msk _ _) eqn: Emsk; cycle 1.
+        { cStepsS. bsimpl. cForceS 0. cStepsS. bsimpl.
+          cForceS. iSplit; et. cStepsS. erewrite Emsk; et. cStepsS. ss.
+        }
+        destruct spt.2 eqn: Espt; cycle 1.
+        { erewrite SP2 in Emsk; et; ss. }
+        cStepsS. cStepsT. bsimpl.
+        cStepsT. cForceS _q. cStepsS. bsimpl.
+        cStepsT. cForcesS. iFrame. cStepsS. des_if; [|cStepsS; ss].
+        cStep. cStepsS. cStepsT. des_if; [|cStepsS; ss].
+        cStepsS. cForceT. iFrame. cStepsT.
+        cByCoind CIH; try et. iFrame "IST WINV".
+    - rewrite !SRed._bind !SRed._pg. destruct s as [k v|k].
+      + cStepsS. cStepsT. des_ifs; [|cStepsS; ss].
+        cStepsS. cStepsT.
+        iApply (wsim_sput_eq _ _
+          (S := list_to_set (Mod.scopes (SMod.to_mod spt md)))).
+        { rewrite elem_of_list_to_set /=. eapply HPUT.
+          rewrite orb_false_r in Heq. exact Heq. }
+        iFrame "IST". iIntros "IST".
+        cStepsS. cStepsT.
+        cByCoind CIH; try et. iFrame "IST WINV".
+      + cStepsS. cStepsT. des_ifs; [|cStepsS; ss].
+        cStepsS. cStepsT.
+        iApply (wsim_sget_eq _ _
+          (S := list_to_set (Mod.scopes (SMod.to_mod spt md)))).
+        { rewrite elem_of_list_to_set /=. eapply HGET.
+          rewrite orb_false_r in Heq. exact Heq. }
+        iFrame "IST". iIntros (?) "IST".
+        cStepsS. cStepsT.
+        cByCoind CIH; try et. iFrame "IST WINV".
+    - rewrite !SRed._bind !SRed._core. destruct e.
+      + cStepsS. cStepsT. des_if; [|cStepsS; ss].
+        cStepsT. cForceS _q. cStepsS.
+        cByCoind CIH; try et. iFrame "IST WINV".
+      + cStepsS. cStepsT. des_if; [|cStepsS; ss].
+        cStepsS. cForceT _q. cStepsT.
+        cByCoind CIH; try et. iFrame "IST WINV".
+      + cStepsS. cStepsT. des_if; [|cStepsS; ss].
+        cStep. cStepsS. cStepsT.
+        cByCoind CIH; try et. iFrame "IST WINV".
+  Qed.
+
+End PREPARE_SIM.
